theories/tree_borrows/defs.v
@@ -3,7 +3,7 @@
 *)
 
 From iris.prelude Require Export prelude.
-From simuliris.tree_borrows Require Export tactics notation lang bor_semantics.
+From simuliris.tree_borrows Require Export tactics notation lang bor_semantics bor_lemmas.
 From iris.prelude Require Import options.
 
 (* Henceforth also in the files importing us we want to use Z_scope. *)
@@ -24,6 +24,8 @@ Record item_wf (it:item) (nxtp:tag) (nxtc:call_id) := {
   item_perm_reachable : it.(initp) ≠ Disabled → map_Forall (λ k v, reach it.(initp) (perm v)) it.(iperm)
 }.
 
+Definition item_all_more_init itp itc := ∀ l, initialized (item_lookup itc l) = PermInit → initialized (item_lookup itp l) = PermInit.
+Definition parents_more_init (tr : tree item) := ∀ tg, every_child tg item_all_more_init tr.
 
 Definition tree_items_unique (tr:tree item) :=
   forall tg,
@@ -38,6 +40,8 @@ Definition wf_tree (tr:tree item) :=
   tree_items_unique tr.
 Definition each_tree_wf (trs:trees) :=
   ∀ blk tr, trs !! blk = Some tr → wf_tree tr.
+Definition each_tree_parents_more_init (trs:trees) :=
+  ∀ blk tr, trs !! blk = Some tr → parents_more_init tr.
 Definition tags_unique_per_location (trs:trees) :=
   ∀ blk1 blk2 tr1 tr2 tg, trs !! blk1 = Some tr1 → trs !! blk2 = Some tr2 →
           tree_contains tg tr1 → tree_contains tg tr2 → blk1 = blk2.
@@ -70,6 +74,7 @@ Record state_wf (s: state) := {
   state_wf_dom : same_blocks s.(shp) s.(strs);
   (*state_wf_mem_tag : wf_mem_tag s.(shp) s.(snp);*) (* FIXME: this seems to state that all pointers are wf, it should be included *)
   state_wf_tree_unq : wf_trees s.(strs);
+  state_wf_tree_more_init : each_tree_parents_more_init s.(strs);
   state_wf_tree_compat : trees_compat_nexts s.(strs) s.(snp) s.(snc);
   state_wf_non_empty : wf_non_empty s.(strs);
   (*state_wf_cid_no_dup : NoDup s.(scs) ;*) (* FIXME: call ids are unique, include this *)
